sketched new hasType paradigm

Pullback/P/Basic.lean
@@ -178,14 +178,21 @@ def RawPExpr.toPExpr {BaseType Const} [DecidableEq BaseType] [Typed Const (PType
     PExpr.letE v' (body.toPExpr ((x, vT)::ctxRaw) hbody)
 | const c, he => .const c
 
-class HasType {Const BaseType} [DecidableEq BaseType] [Typed Const (PType BaseType)] (ctxRaw : List (Name × PType BaseType)) (e : RawPExpr (Const := Const) (BaseType := BaseType)) (ty : outParam (PType BaseType)) where
-  hasType : e.inferType ctxRaw = ty
+def RawPExpr.hasType {Const BaseType} [DecidableEq BaseType] [Typed Const (PType BaseType)] (ctxRaw : List (Name × PType BaseType)) (e : RawPExpr Const BaseType) (ty : (PType BaseType)) : Prop :=
+  e.inferType ctxRaw = ty -- todo make this recursive and not use inferType (to avoid Option hell)
+
+theorem RawPExpr.hasType_iff_inferType_eq_some {Const BaseType} [DecidableEq BaseType] [Typed Const (PType BaseType)] (ctxRaw : List (Name × PType BaseType)) (e : RawPExpr Const BaseType) (ty : (PType BaseType)) :
+    e.hasType ctxRaw ty ↔ e.inferType ctxRaw = ty := by
+  rfl -- this proof will need to be updated when hasType is defined recursively
+
+class HasType {Const BaseType} [DecidableEq BaseType] [Typed Const (PType BaseType)] (ctxRaw : List (Name × PType BaseType)) (e : RawPExpr Const BaseType) (ty : outParam (PType BaseType)) where
+  hasType : e.hasType ctxRaw ty
 
 def RawPExpr.toPExpr' {BaseType Const} [DecidableEq BaseType] [Typed Const (PType BaseType)] (ctxRaw : List (Name × PType BaseType)) (ty : PType BaseType) :
   (e : RawPExpr Const BaseType) → [HasType ctxRaw e ty] →
     (PExpr Const BaseType (ctxRaw.map (·.2)) ty) :=
   fun e he =>
-    cast (by grind [HasType]) (e.toPExpr ctxRaw (by grind [HasType]))
+    cast (by grind [HasType, hasType]) (e.toPExpr ctxRaw (by grind [HasType, hasType]))
 
 namespace RawPExpr
 
@@ -194,11 +201,11 @@ variable {BaseType Const} [DecidableEq BaseType] [Typed Const (PType BaseType)]
 theorem hasType_var (ty : PType BaseType) (ctxRaw : List (Name × PType BaseType)) (name : Name)
     (hname : (ctxRaw.find? (·.1 == name)) = some (name, ty)) :
   HasType ctxRaw (RawPExpr.var name : RawPExpr Const BaseType) ty :=
-  ⟨by simpa [inferType] using congrArg (Option.map Prod.snd) hname⟩
+  ⟨by simpa [inferType, hasType] using congrArg (Option.map Prod.snd) hname⟩
 
 instance instHasType_const (ctxRaw : List (Name × PType BaseType)) (c : Const) :
   HasType ctxRaw (RawPExpr.const c : RawPExpr Const BaseType) (Typed.type c) :=
-  ⟨by simp [inferType]⟩
+  ⟨by simp [inferType, hasType]⟩
 
 instance instHasType_lam (ctxRaw : List (Name × PType BaseType)) (x : Name) (argT bodyT : PType BaseType)
     (body : RawPExpr Const BaseType) [HasType ((x, argT)::ctxRaw) body bodyT] :
@@ -206,7 +213,7 @@ instance instHasType_lam (ctxRaw : List (Name × PType BaseType)) (x : Name) (ar
   ⟨by
     have hbody : inferType ((x, argT) :: ctxRaw) body = some bodyT :=
       HasType.hasType (ctxRaw := ((x, argT) :: ctxRaw)) (e := body) (ty := bodyT)
-    simp [inferType, hbody]
+    simp [inferType, hbody, hasType]
   ⟩
 
 instance instHasType_letE (ctxRaw : List (Name × PType BaseType)) (x : Name)
@@ -218,10 +225,10 @@ instance instHasType_letE (ctxRaw : List (Name × PType BaseType)) (x : Name)
       HasType.hasType (ctxRaw := ctxRaw) (e := v) (ty := vT)
     have hbody : inferType ((x, vT) :: ctxRaw) body = some bodyT :=
       HasType.hasType (ctxRaw := ((x, vT) :: ctxRaw)) (e := body) (ty := bodyT)
-    simp [inferType, hv, hbody]
+    simp [inferType, hv, hbody, hasType]
   ⟩
 
 instance instHasType_app (ctxRaw : List (Name × PType BaseType)) (dom codom : PType BaseType) (f x : RawPExpr Const BaseType) [HasType ctxRaw f (PType.fun dom codom)] [HasType ctxRaw x dom] :
   HasType ctxRaw (RawPExpr.app f x) codom :=
-  ⟨by simp [inferType]; grind [HasType]⟩
+  ⟨by simp [inferType, hasType]; grind [HasType, hasType]⟩
 end RawPExpr
